wip

src/day02.lean
@@ -1,5 +1,5 @@
 import system.io data.buffer.parser
-open parser
+open parser nat
 
 def go {α} (file : string) (p : parser α) (m: α → option string) : io unit :=
 do s ← io.fs.read_file file,
@@ -10,3 +10,26 @@ do s ← io.fs.read_file file,
 def parse_number := string.to_nat <$> many_char1 (sat char.is_digit)
 
 def day1 := go "day02.txt" (many (parse_number <* ch ','))
+
+lemma foo {n m : ℕ} (h: n ≤ m) (x : fin n) : x.val < m :=
+let hx: x.val < n := x.is_lt in
+lt_of_lt_of_le hx h
+
+lemma le_plus_four {n : ℕ} : n ≤ n + 4 :=
+less_than_or_equal.step $ less_than_or_equal.step $ less_than_or_equal.step $ less_than_or_equal.step $ less_than_or_equal.refl n
+
+def coerce_fin {n m : ℕ} : ( n ≤ m ) → fin n → fin m
+| hleq x := ⟨ x.val, foo hleq x ⟩
+
+-- map current memory, current pointer, to new memory, and flag for done or not
+def step (s: ℕ) : (array (s + 4) ℕ) → fin s → ((array (s + 4) ℕ) × bool)
+| m idx :=
+let current := m.read (coerce_fin le_plus_four idx)  in
+if current = 99 then ⟨ m, true ⟩
+else if current = 1 then sorry
+else sorry
+
+
+#check (⟨λ _, 0⟩: array 60 ℕ)
+
+
